cedar-lean/Cedar/Thm/SymCC/Compiler.lean
@@ -24,7 +24,6 @@ import Cedar.Thm.SymCC.Compiler.LitVar
 import Cedar.Thm.SymCC.Compiler.Record
 import Cedar.Thm.SymCC.Compiler.Set
 import Cedar.Thm.SymCC.Compiler.Unary
-import Cedar.Thm.SymCC.Compiler.WellTyped
 
 /-!
 This file proves two key auxiliary lemmas used to show the soundness
